lib/Encoding.ml
@@ -1,0 +1,50 @@
+open Maps
+open RelocProgram
+open Camlcoq
+    
+let char_of_byte i =
+  if 32 <= i && i <= 126
+  then Char.chr i else '.'
+
+let rec take_drop n l =
+  match n, l with
+  | 0, l -> ([],l)
+  | _, h::t ->
+    let (l1, l2) = take_drop (n-1) t in
+    (h::l1, l2)
+  | _, [] -> ([],[])
+
+let rec dump_bytes sbytes : unit =
+  if sbytes = [] then ()
+  else
+    begin
+      let (l1,l2) = take_drop 16 sbytes in
+      Printf.printf "%s %s\n"
+        (String.concat " " (List.map (fun i -> Printf.sprintf "%02x" i)l1))
+        (String.concat "" (List.map (fun i -> Printf.sprintf "%c" (char_of_byte i))l1));
+      dump_bytes l2
+    end
+
+let dump_bytes sbytes =
+  let sbytes = List.map (fun b -> Camlcoq.Z.to_int (Integers.Byte.unsigned b)) sbytes in
+  dump_bytes sbytes
+
+
+
+
+let dump_strmap strmap : unit =
+  let elts = PTree.elements strmap in
+  let elts = List.map (fun (pkey, zofs) -> (Camlcoq.extern_atom pkey, Camlcoq.Z.to_int zofs)) elts in
+  let elts = List.sort (fun e1 e2 -> compare (snd e1) (snd e2)) elts in
+  List.iter (fun (str, ofs) -> Printf.printf "%s -> %d\n" str ofs) elts
+
+
+let dump_symtable symt =
+  List.iteri (fun i symt_entry ->
+      let id = match symbentry_id symt_entry with
+          Some x -> x
+        | _ -> BinNums.Coq_xH in
+      let zid = Camlcoq.P.to_int id in
+      let s = extern_atom id in
+      Printf.printf "%02d: %d '%s'\n" i zid s
+    ) symt
